fix names for label, mode, and transition

theory/Static_Communication.thy
@@ -4,30 +4,30 @@ theory Static_Communication
     Dynamic_Communication
 begin
 
-datatype node_label = NLet var | NResult var
+datatype label = NLet var | NResult var
 
-fun top_node_label :: "exp \<Rightarrow> node_label" where
-  "top_node_label (Let x b e) = NLet x" |
-  "top_node_label (Rslt y) = NResult y"
+fun top_label :: "exp \<Rightarrow> label" where
+  "top_label (Let x b e) = NLet x" |
+  "top_label (Rslt y) = NResult y"
 
-type_synonym node_set = "node_label set"
+type_synonym label_set = "label set"
 
-type_synonym node_map = "node_label \<Rightarrow> var set"
+type_synonym label_map = "label \<Rightarrow> var set"
 
-inductive static_send_node_label :: "abstract_env \<Rightarrow> exp \<Rightarrow> var \<Rightarrow> node_label \<Rightarrow> bool" where
+inductive static_send_label :: "abstract_env \<Rightarrow> exp \<Rightarrow> var \<Rightarrow> label \<Rightarrow> bool" where
   intro: "
     {^Chan xC} \<subseteq> V xSC \<Longrightarrow>
     {^SendEvt xSC xM} \<subseteq> V xE \<Longrightarrow>
     static_reachable e (Let x (Sync xE) e') \<Longrightarrow>
-    static_send_node_label V e xC (NLet x)
+    static_send_label V e xC (NLet x)
   "
 
-inductive static_recv_node_label :: "abstract_env \<Rightarrow> exp \<Rightarrow> var \<Rightarrow> node_label \<Rightarrow> bool" where
+inductive static_recv_label :: "abstract_env \<Rightarrow> exp \<Rightarrow> var \<Rightarrow> label \<Rightarrow> bool" where
   intro: "
     {^Chan xC} \<subseteq> V xRC \<Longrightarrow>
     {^RecvEvt xRC} \<subseteq> V xE \<Longrightarrow>
     static_reachable e (Let x (Sync xE) e') \<Longrightarrow>
-    static_recv_node_label V e xC (NLet x)
+    static_recv_label V e xC (NLet x)
   "
 
 end
