theory/Static_Communication_A.thy
@@ -6,73 +6,73 @@ theory Static_Communication_A
     Static_Communication
 begin
 
-datatype edge_label = ENext | ESpawn | ECall | EReturn
+datatype mode = ENext | ESpawn | ECall | EReturn
 
-type_synonym flow_label = "(node_label \<times> edge_label \<times> node_label)"
+type_synonym transition = "(label \<times> mode \<times> label)"
 
-type_synonym flow_set = "flow_label set"
+type_synonym transition_set = "transition set"
 
-type_synonym step_label = "(node_label \<times> edge_label)"
+type_synonym step = "(label \<times> mode)"
 
-type_synonym abstract_path = "step_label list"
+type_synonym abstract_path = "step list"
 
 
-inductive static_traversable :: "abstract_env \<Rightarrow> flow_set \<Rightarrow> exp \<Rightarrow> bool"  where
+inductive static_traversable :: "abstract_env \<Rightarrow> transition_set \<Rightarrow> exp \<Rightarrow> bool"  where
   Result: "
     static_traversable V F (Rslt x)
   " |
   Let_Unit: "
     \<lbrakk>
-      {(NLet x , ENext, top_node_label e)} \<subseteq> F;
+      {(NLet x , ENext, top_label e)} \<subseteq> F;
       static_traversable V F e
     \<rbrakk> \<Longrightarrow>
     static_traversable V F (Let x Unt e)
   " |
   Let_Chan: "
     \<lbrakk>
-      {(NLet x, ENext, top_node_label e)} \<subseteq> F;
+      {(NLet x, ENext, top_label e)} \<subseteq> F;
       static_traversable V F e
     \<rbrakk> \<Longrightarrow>
     static_traversable V F (Let x MkChn e)
   " |
   Let_SendEvt: "
     \<lbrakk>
-      {(NLet x, ENext, top_node_label e)} \<subseteq> F;
+      {(NLet x, ENext, top_label e)} \<subseteq> F;
       static_traversable V F e
     \<rbrakk> \<Longrightarrow>
     static_traversable V F (Let x (Prim (SendEvt x\<^sub>c x\<^sub>m)) e)
   " |
   Let_RecvEvt: "
     \<lbrakk>
-      {(NLet x, ENext, top_node_label e)} \<subseteq> F;
+      {(NLet x, ENext, top_label e)} \<subseteq> F;
       static_traversable V F e
     \<rbrakk> \<Longrightarrow>
     static_traversable V F (Let x (Prim (RecvEvt x\<^sub>c)) e)
   " |
   Let_Pair: "
     \<lbrakk>
-      {(NLet x, ENext, top_node_label e)} \<subseteq> F;
+      {(NLet x, ENext, top_label e)} \<subseteq> F;
       static_traversable V F e
     \<rbrakk> \<Longrightarrow>
     static_traversable V F (Let x (Prim (Pair x\<^sub>1 x\<^sub>2)) e)
   " |
   Let_Left: "
     \<lbrakk>
-      {(NLet x, ENext, top_node_label e)} \<subseteq> F;
+      {(NLet x, ENext, top_label e)} \<subseteq> F;
       static_traversable V F e
     \<rbrakk> \<Longrightarrow>
     static_traversable V F (Let x (Prim (Lft x\<^sub>p)) e)
   " |
   Let_Right: "
     \<lbrakk>
-      {(NLet x, ENext, top_node_label e)} \<subseteq> F;
+      {(NLet x, ENext, top_label e)} \<subseteq> F;
       static_traversable V F e
     \<rbrakk> \<Longrightarrow>
     static_traversable V F (Let x (Prim (Rght x\<^sub>p)) e)
   " |
   Let_Abs: "
     \<lbrakk>
-      {(NLet x, ENext, top_node_label e)} \<subseteq> F;
+      {(NLet x, ENext, top_label e)} \<subseteq> F;
       static_traversable V F e\<^sub>b;
       static_traversable V F e
     \<rbrakk> \<Longrightarrow>
@@ -81,8 +81,8 @@ inductive static_traversable :: "abstract_env \<Rightarrow> flow_set \<Rightarro
   Let_Spawn: "
     \<lbrakk>
       {
-        (NLet x, ENext, top_node_label e),
-        (NLet x, ESpawn, top_node_label e\<^sub>c)
+        (NLet x, ENext, top_label e),
+        (NLet x, ESpawn, top_label e\<^sub>c)
       } \<subseteq> F;
       static_traversable V F e\<^sub>c;
       static_traversable V F e
@@ -91,21 +91,21 @@ inductive static_traversable :: "abstract_env \<Rightarrow> flow_set \<Rightarro
   " |
   Let_Sync: "
     \<lbrakk>
-      {(NLet x, ENext, top_node_label e)} \<subseteq> F;
+      {(NLet x, ENext, top_label e)} \<subseteq> F;
       static_traversable V F e
     \<rbrakk> \<Longrightarrow>
     static_traversable V F (Let x (Sync xSE) e)
   " |
   Let_Fst: "
     \<lbrakk>
-      {(NLet x, ENext, top_node_label e)} \<subseteq> F;
+      {(NLet x, ENext, top_label e)} \<subseteq> F;
       static_traversable V F e
     \<rbrakk> \<Longrightarrow>
     static_traversable V F (Let x (Fst x\<^sub>p) e)
   " |
   Let_Snd: "
     \<lbrakk>
-      {(NLet x, ENext, top_node_label e)} \<subseteq> F;
+      {(NLet x, ENext, top_label e)} \<subseteq> F;
       static_traversable V F e
     \<rbrakk> \<Longrightarrow>
     static_traversable V F (Let x (Snd x\<^sub>p) e)
@@ -113,10 +113,10 @@ inductive static_traversable :: "abstract_env \<Rightarrow> flow_set \<Rightarro
   Let_Case: "
     \<lbrakk>
       {
-        (NLet x, ECall, top_node_label e\<^sub>l),
-        (NLet x, ECall, top_node_label e\<^sub>r),
-        (NResult (\<lfloor>e\<^sub>l\<rfloor>), EReturn, top_node_label e),
-        (NResult (\<lfloor>e\<^sub>r\<rfloor>), EReturn, top_node_label e)
+        (NLet x, ECall, top_label e\<^sub>l),
+        (NLet x, ECall, top_label e\<^sub>r),
+        (NResult (\<lfloor>e\<^sub>l\<rfloor>), EReturn, top_label e),
+        (NResult (\<lfloor>e\<^sub>r\<rfloor>), EReturn, top_label e)
       } \<subseteq> F;
       static_traversable V F e\<^sub>l;
       static_traversable V F e\<^sub>r;
@@ -128,8 +128,8 @@ inductive static_traversable :: "abstract_env \<Rightarrow> flow_set \<Rightarro
     \<lbrakk>
       (\<forall> f' x\<^sub>p e\<^sub>b . ^Abs f' x\<^sub>p e\<^sub>b \<in> V f \<longrightarrow>
         {
-          (NLet x, ECall, top_node_label e\<^sub>b),
-          (NResult (\<lfloor>e\<^sub>b\<rfloor>), EReturn, top_node_label e)
+          (NLet x, ECall, top_label e\<^sub>b),
+          (NResult (\<lfloor>e\<^sub>b\<rfloor>), EReturn, top_label e)
         } \<subseteq> F);
       static_traversable V F e
     \<rbrakk> \<Longrightarrow>
@@ -138,7 +138,7 @@ inductive static_traversable :: "abstract_env \<Rightarrow> flow_set \<Rightarro
 
 
 
-inductive static_traceable :: "abstract_env \<Rightarrow> flow_set \<Rightarrow> node_label \<Rightarrow> (node_label \<Rightarrow> bool) \<Rightarrow> abstract_path \<Rightarrow> bool" where
+inductive static_traceable :: "abstract_env \<Rightarrow> transition_set \<Rightarrow> label \<Rightarrow> (label \<Rightarrow> bool) \<Rightarrow> abstract_path \<Rightarrow> bool" where
   Empty: "
     isEnd start \<Longrightarrow>
     static_traceable V F start isEnd []
@@ -194,29 +194,29 @@ inductive noncompetitive :: "abstract_path \<Rightarrow> abstract_path \<Rightar
 
 inductive static_one_shot :: "abstract_env \<Rightarrow> exp \<Rightarrow> var \<Rightarrow> bool" where
   Sync: "
-    every_two (static_traceable V F (top_node_label e) (static_send_node_label V e xC)) singular \<Longrightarrow>
+    every_two (static_traceable V F (top_label e) (static_send_label V e xC)) singular \<Longrightarrow>
     static_traversable V F e \<Longrightarrow>
     static_one_shot V e xC 
   "
 
 inductive static_one_to_one :: "abstract_env \<Rightarrow> exp \<Rightarrow> var \<Rightarrow> bool" where
   Sync: "
-    every_two (static_traceable V F (top_node_label e) (static_send_node_label V e xC)) noncompetitive \<Longrightarrow>
-    every_two (static_traceable V F (top_node_label e) (static_recv_node_label V e xC)) noncompetitive \<Longrightarrow>
+    every_two (static_traceable V F (top_label e) (static_send_label V e xC)) noncompetitive \<Longrightarrow>
+    every_two (static_traceable V F (top_label e) (static_recv_label V e xC)) noncompetitive \<Longrightarrow>
     static_traversable V F e \<Longrightarrow>
     static_one_to_one V e xC 
   "
 
 inductive static_fan_out :: "abstract_env \<Rightarrow> exp \<Rightarrow> var \<Rightarrow> bool" where
   Sync: "
-    every_two (static_traceable V F (top_node_label e) (static_send_node_label V e xC)) noncompetitive \<Longrightarrow>
+    every_two (static_traceable V F (top_label e) (static_send_label V e xC)) noncompetitive \<Longrightarrow>
     static_traversable V F e \<Longrightarrow>
     static_fan_out V e xC 
   "
 
 inductive static_fan_in :: "abstract_env \<Rightarrow> exp \<Rightarrow> var \<Rightarrow> bool" where
   Sync: "
-    every_two (static_traceable V F (top_node_label e) (static_recv_node_label V e xC)) noncompetitive \<Longrightarrow>
+    every_two (static_traceable V F (top_label e) (static_recv_label V e xC)) noncompetitive \<Longrightarrow>
     static_traversable V F e \<Longrightarrow>
     static_fan_in V e xC 
   "
